src/coq/Semantics/InfiniteToFinite.v
@@ -1,2 +1,12 @@
 From Vellvm Require Import
+     Semantics.InterpretationStack
+     Semantics.LLVMEvents
+     Semantics.Denotation
+     Semantics.MemoryAddress
+     Semantics.Memory.Sizeof
+     Semantics.Lang
      Semantics.InterpretationStack.
+
+Module Type InfiniteToFinite (LLVM1 : InterpreterStack) (LLVM2 : InterpreterStack).
+  (* Parameter oom_refine : LLVM1. *)
+End InfiniteToFinite.
