src/coq/Semantics/LLVMParams.v
@@ -1,0 +1,28 @@
+From Vellvm Require Import
+     Semantics.MemoryAddress
+     Semantics.Memory.Sizeof.
+
+(** Parameters for LLVM instances. *)
+Module Type LLVMParams.
+  Declare Module ADDR : ADDRESS.
+  Declare Module IP : INTPTR.
+  Declare Module SIZEOF : Sizeof.
+  Declare Module PTOI : PTOI ADDR.
+  Declare Module PROV : PROVENANCE ADDR.
+  Declare Module ITOP : ITOP ADDR PROV.
+End LLVMParams.
+
+Module Make (ADDR' : ADDRESS) (IP' : INTPTR) (SIZEOF' : Sizeof) (PTOI' : PTOI ADDR') (PROV' : PROVENANCE ADDR') (ITOP' : ITOP ADDR' PROV') : LLVMParams.
+  Module ADDR := ADDR'.
+  Module IP := IP'.
+  Module SIZEOF := SIZEOF'.
+  Module PTOI := PTOI'.
+  Module PROV := PROV'.
+  Module ITOP := ITOP'.
+End Make.
+
+(*
+Module LLVMParamsBigIntptr := Make FiniteMemory.Addr FiniteMemory.BigIP FiniteMemory.FinSizeof FiniteMemory.FinPTOI FiniteMemory.FinPROV FiniteMemory.FinITOP.
+
+Module LLVMParams64BitIntptr := Make FiniteMemory.Addr FiniteMemory.IP64Bit FiniteMemory.FinSizeof FiniteMemory.FinPTOI FiniteMemory.FinPROV FiniteMemory.FinITOP.
+*)
