src/coq/Semantics/TopLevel.v
@@ -30,12 +30,12 @@ From Vellvm Require Import
      Semantics.Denotation
      Semantics.IntrinsicsDefinitions
      Handlers.Handlers
-     Semantics.InterpretationStack.
+     Semantics.InterpretationStack
+     Semantics.LLVMParams.
 
 Import MonadNotation.
 Import ListNotations.
 Import Monads.
-Import SemNotations.
 Open Scope string_scope.
 
 (* end hide *)
@@ -52,89 +52,44 @@ Open Scope string_scope.
    by setting its bits to 0.
  *)
 
-(** * Initialization
+Module Type LLVMTopLevel.
+  Declare Module IS : InterpreterStack.
+
+  Export IS.
+
+  Import SemNotations.
+
+  (** * Initialization
     The initialization phase allocates and initializes globals,
     and allocates function pointers. This initialization phase is internalized
     in [Vellvm], it is an [itree] as any other.
- *)
+   *)
 
-Definition allocate_global (g:global dtyp) : itree L0 unit :=
-  'v <- trigger (Alloca (g_typ g));;
-  trigger (GlobalWrite (g_ident g) v).
+  Parameter allocate_global : global dtyp -> itree L0 unit.
+  Parameter allocate_globals : list (global dtyp) -> itree L0 unit.
 
-Definition allocate_globals (gs:list (global dtyp)) : itree L0 unit :=
-  map_monad_ allocate_global gs.
+  (* Who is in charge of allocating the addresses for external functions declared in this mcfg? *)
 
-(* Who is in charge of allocating the addresses for external functions declared in this mcfg? *)
+  (* Returns `true` only if both function are named and have the same name.  *)
+  Parameter function_name_eq : function_id -> function_id -> bool.
 
-(* Returns `true` only if both function are named and have the same name.  *)
-Definition function_name_eq (a b:function_id) : bool :=
-  match a, b with
-  | Name aname, Name bname => eqb aname bname
-  | _, _ => false
-  end.
+  Parameter allocate_declaration : declaration dtyp -> itree L0 unit.
+  Parameter allocate_declarations : list (declaration dtyp) -> itree L0 unit.
 
-Definition allocate_declaration (d:declaration dtyp) : itree L0 unit :=
-  match List.find (fun x => function_name_eq (dc_name d) (dc_name x)) defined_intrinsics_decls with
-  | Some _ => Ret tt (* Don't allocate pointers for LLVM intrinsics declarations *)
-  | None =>
-    'v <- trigger (Alloca DTYPE_Pointer);;
-    trigger (GlobalWrite (dc_name d) v)
-  end.
+  Parameter initialize_global : global dtyp -> itree exp_E unit.
+  Parameter initialize_globals : list (global dtyp) -> itree exp_E unit.
 
-Definition allocate_declarations (ds:list (declaration dtyp)) : itree L0 unit :=
-  map_monad_ allocate_declaration ds.
+  Parameter build_global_environment : CFG.mcfg dtyp -> itree L0 unit.
 
-Definition initialize_global (g:global dtyp) : itree exp_E unit :=
-  let dt := (g_typ g) in
-  a <- trigger (GlobalRead (g_ident g));;
-  uv <- match (g_exp g) with
-       | None => ret (UVALUE_Undef dt)
-       | Some e =>  ⟦ e at dt ⟧e
-       end ;;
-  trigger (Store dt a uv).
+  Parameter function_env : Type.
+  Parameter address_one_function : definition dtyp (CFG.cfg dtyp) -> itree L0 (dvalue * function_denotation).
 
-Definition initialize_globals (gs:list (global dtyp)): itree exp_E unit :=
-  map_monad_ initialize_global gs.
+  Notation res_L1 := (global_env * uvalue)%type.
+  Notation res_L2 := (local_env * lstack * res_L1)%type.
+  Notation res_L3 := (MemState * res_L2)%type.
+  Notation res_L4 := (MemState * (local_env * lstack * (global_env * uvalue)))%type.
 
-Definition build_global_environment (CFG : CFG.mcfg dtyp) : itree L0 unit :=
-  allocate_declarations ((m_declarations CFG) ++ (List.map (df_prototype) (m_definitions CFG)));;
-  allocate_globals (m_globals CFG) ;;
-  translate exp_to_L0 (initialize_globals (m_globals CFG)).
-
-(** Local environment implementation
-    The map-based handlers are defined parameterized over a domain of key and value.
-    We now pick concrete such domain.
-    Note that while local environments may store under-defined values,
-    global environments are statically guaranteed to store [dvalue]s.
- *)
-Definition function_env := FMapAList.alist dvalue D.function_denotation.
-
-(**
-   Denotes a function and returns its pointer.
- *)
-
-Definition address_one_function (df : definition dtyp (CFG.cfg dtyp)) : itree L0 (dvalue * D.function_denotation) :=
-  let fid := (dc_name (df_prototype df)) in
-  fv <- trigger (GlobalRead fid) ;;
-  ret (fv, ⟦ df ⟧f).
-
-(**
-   We are now ready to define our semantics. Guided by the events and handlers,
-   we work in layers: the first layer is defined as the uninterpreted [itree]
-   resulting from the denotation of the LLVM program. Each successive handler
-   then transform a tree at layer n to a tree at layer (n+1).
- *)
-(**
-   In order to limit bloated type signature, we name the successive return types.
- *)
-
-Notation res_L1 := (global_env * uvalue)%type.
-Notation res_L2 := (local_env * lstack * res_L1)%type.
-Notation res_L3 := (MemState * res_L2)%type.
-Notation res_L4 := (MemState * (local_env * lstack * (global_env * uvalue)))%type.
-
-(**
+  (**
      Full denotation of a Vellvm program as an interaction tree:
      * initialize the global environment;
      * point wise denote each function;
@@ -148,71 +103,216 @@ Notation res_L4 := (MemState * (local_env * lstack * (global_env * uvalue)))%typ
      *  %ans = call ret_typ entry (args)
      *  ret ret_typ %ans
      *)
-Definition denote_vellvm
-           (ret_typ : dtyp)
-           (entry : string)
-           (args : list uvalue)
-           (mcfg : CFG.mcfg dtyp) : itree L0 uvalue :=
-  build_global_environment mcfg ;;
-  'defns <- map_monad address_one_function (m_definitions mcfg) ;;
-  'addr <- trigger (GlobalRead (Name entry)) ;;
-  denote_mcfg defns ret_typ (dvalue_to_uvalue addr) args.
+  Parameter denote_vellvm :
+    dtyp ->
+    string ->
+    list uvalue ->
+    CFG.mcfg dtyp ->
+    itree L0 uvalue.
+
+  Parameter main_args : list uvalue.
+
+  Parameter denote_vellvm_main : CFG.mcfg dtyp -> itree L0 uvalue.
+
+  Parameter interpreter_gen :
+    dtyp ->
+    string ->
+    list uvalue ->
+    list (toplevel_entity typ (block typ * list (block typ))) ->
+    itree L6_exec res_L4.
+
+  Parameter interpreter :
+    list (toplevel_entity typ (block typ * list (block typ))) ->
+    itree L6_exec res_L4.
+
+  Parameter model_gen :
+    dtyp ->
+    string ->
+    list uvalue ->
+    list (toplevel_entity typ (block typ * list (block typ))) ->
+    PropT L6 (MemState * (local_env * lstack * (global_env * uvalue))).
+
+  Parameter model :
+    list (toplevel_entity typ (block typ * list (block typ))) ->
+    PropT L6 res_L4.
+End LLVMTopLevel.
+
+Module Make (IS' : InterpreterStack) : LLVMTopLevel.
+  Module IS := IS'.
+
+  Export IS.
+  Export IS.LLVM.Events.
+  Export IS.LLVM.D.
+  Export IS.LLVM.MEM.
+  Export IS.LLVM.Local.
+  Export IS.LLVM.Global.
+  Export IS.LLVM.Stack.
+  Export IS.LP.ADDR.
+
+  Import SemNotations.
+
+  (** * Initialization
+    The initialization phase allocates and initializes globals,
+    and allocates function pointers. This initialization phase is internalized
+    in [Vellvm], it is an [itree] as any other.
+   *)
+
+  Definition allocate_global (g:global dtyp) : itree L0 unit :=
+    'v <- trigger (Alloca (g_typ g));;
+    trigger (GlobalWrite (g_ident g) v).
+
+  Definition allocate_globals (gs:list (global dtyp)) : itree L0 unit :=
+    map_monad_ allocate_global gs.
+
+  (* Who is in charge of allocating the addresses for external functions declared in this mcfg? *)
+
+  (* Returns `true` only if both function are named and have the same name.  *)
+  Definition function_name_eq (a b:function_id) : bool :=
+    match a, b with
+    | Name aname, Name bname => eqb aname bname
+    | _, _ => false
+    end.
+
+  Definition allocate_declaration (d:declaration dtyp) : itree L0 unit :=
+    match List.find (fun x => function_name_eq (dc_name d) (dc_name x)) defined_intrinsics_decls with
+    | Some _ => Ret tt (* Don't allocate pointers for LLVM intrinsics declarations *)
+    | None =>
+        'v <- trigger (Alloca DTYPE_Pointer);;
+        trigger (GlobalWrite (dc_name d) v)
+    end.
+
+  Definition allocate_declarations (ds:list (declaration dtyp)) : itree L0 unit :=
+    map_monad_ allocate_declaration ds.
+
+  Definition initialize_global (g:global dtyp) : itree exp_E unit :=
+    let dt := (g_typ g) in
+    a <- trigger (GlobalRead (g_ident g));;
+    uv <- match (g_exp g) with
+         | None => ret (UVALUE_Undef dt)
+         | Some e =>  ⟦ e at dt ⟧e
+         end ;;
+    trigger (Store dt a uv).
+
+  Definition initialize_globals (gs:list (global dtyp)): itree exp_E unit :=
+    map_monad_ initialize_global gs.
+
+  Definition build_global_environment (CFG : CFG.mcfg dtyp) : itree L0 unit :=
+    allocate_declarations ((m_declarations CFG) ++ (List.map (df_prototype) (m_definitions CFG)));;
+    allocate_globals (m_globals CFG) ;;
+    translate exp_to_L0 (initialize_globals (m_globals CFG)).
+
+  (** Local environment implementation
+    The map-based handlers are defined parameterized over a domain of key and value.
+    We now pick concrete such domain.
+    Note that while local environments may store under-defined values,
+    global environments are statically guaranteed to store [dvalue]s.
+   *)
+  Definition function_env := FMapAList.alist dvalue function_denotation.
+
+  (**
+   Denotes a function and returns its pointer.
+   *)
+
+  Definition address_one_function (df : definition dtyp (CFG.cfg dtyp)) : itree L0 (dvalue * function_denotation) :=
+    let fid := (dc_name (df_prototype df)) in
+    fv <- trigger (GlobalRead fid) ;;
+    ret (fv, ⟦ df ⟧f).
+
+  (**
+   We are now ready to define our semantics. Guided by the events and handlers,
+   we work in layers: the first layer is defined as the uninterpreted [itree]
+   resulting from the denotation of the LLVM program. Each successive handler
+   then transform a tree at layer n to a tree at layer (n+1).
+   *)
+  (**
+   In order to limit bloated type signature, we name the successive return types.
+   *)
+
+  Notation res_L1 := (global_env * uvalue)%type.
+  Notation res_L2 := (local_env * lstack * res_L1)%type.
+  Notation res_L3 := (MemState * res_L2)%type.
+  Notation res_L4 := (MemState * (local_env * lstack * (global_env * uvalue)))%type.
+
+  (**
+     Full denotation of a Vellvm program as an interaction tree:
+     * initialize the global environment;
+     * point wise denote each function;
+     * retrieve the address of the entry point function;
+     * tie the mutually recursive know and run it starting from the 
+     * entry point
+     *
+     * This code should be semantically equivalent to running the following
+     * LLVM snippet after initializing the global configuration:
+     *
+     *  %ans = call ret_typ entry (args)
+     *  ret ret_typ %ans
+     *)
+  Definition denote_vellvm
+             (ret_typ : dtyp)
+             (entry : string)
+             (args : list uvalue)
+             (mcfg : CFG.mcfg dtyp) : itree L0 uvalue :=
+    build_global_environment mcfg ;;
+    'defns <- map_monad address_one_function (m_definitions mcfg) ;;
+    'addr <- trigger (GlobalRead (Name entry)) ;;
+    denote_mcfg defns ret_typ (dvalue_to_uvalue addr) args.
 
 
-(* main_args and denote_vellvm_main may not be needed anymore, but I'm keeping them 
+  (* main_args and denote_vellvm_main may not be needed anymore, but I'm keeping them 
      For backwards compatibility.
- *)
-(* (for now) assume that [main (i64 argc, i8** argv)]
+   *)
+  (* (for now) assume that [main (i64 argc, i8** argv)]
     pass in 0 and null as the arguments to main
     Note: this isn't compliant with standard C semantics
- *)
-Definition main_args := [DV.UVALUE_I64 (DynamicValues.Int64.zero);
-                        DV.UVALUE_Addr (Addr.null)
-                        ].
+   *)
+  Definition main_args := [DV.UVALUE_I64 (DynamicValues.Int64.zero);
+                           DV.UVALUE_Addr null
+    ].
 
-Definition denote_vellvm_main (mcfg : CFG.mcfg dtyp) : itree L0 uvalue :=
-  denote_vellvm (DTYPE_I (32)%N) "main" main_args mcfg.
+  Definition denote_vellvm_main (mcfg : CFG.mcfg dtyp) : itree L0 uvalue :=
+    denote_vellvm (DTYPE_I (32)%N) "main" main_args mcfg.
 
-(**
+  (**
      Now that we know how to denote a whole llvm program, we can _interpret_
      the resulting [itree].
- *)
-Definition interpreter_gen
-           (ret_typ : dtyp)
-           (entry : string)
-           (args : list uvalue)
-           (prog: list (toplevel_entity typ (block typ * list (block typ))))
-  : itree L6_exec res_L4 :=
-  let t := denote_vellvm ret_typ entry args (convert_types (mcfg_of_tle prog)) in
-  interp_mcfg6_exec t [] ([],[]) emptyMemState.
+   *)
+  Definition interpreter_gen
+             (ret_typ : dtyp)
+             (entry : string)
+             (args : list uvalue)
+             (prog: list (toplevel_entity typ (block typ * list (block typ))))
+    : itree L6_exec res_L4 :=
+    let t := denote_vellvm ret_typ entry args (convert_types (mcfg_of_tle prog)) in
+    interp_mcfg6_exec t [] ([],[]) emptyMemState.
 
-(**
+  (**
      Finally, the reference interpreter assumes no user-defined intrinsics and starts 
      from "main" using bogus initial inputs.
- *)
-Definition interpreter := interpreter_gen (DTYPE_I 32%N) "main" main_args.
+   *)
+  Definition interpreter := interpreter_gen (DTYPE_I 32%N) "main" main_args.
 
-(**
+  (**
      We now turn to the definition of our _model_ of vellvm's semantics. The
      process is extremely similar to the one for defining the executable
      semantics, except that we use, where relevant, the handlers capturing
      all allowed behaviors into the [Prop] monad.
- *)
-(**
+   *)
+  (**
      The model simply performs the syntactic conversion from [toplevel_entity]
      to [mcfg], normalizes the types, denotes the [mcfg] and finally interprets the tree
      starting from empty environments.
- *)
-Definition model_gen
-           (ret_typ : dtyp)
-           (entry : string)
-           (args : list uvalue)
-           (prog: list (toplevel_entity typ (block typ * list (block typ))))
-  : PropT L6 (MemState * (local_env * lstack * (global_env * uvalue))) :=
-  let t := denote_vellvm ret_typ entry args (convert_types (mcfg_of_tle prog)) in
-  ℑs eq t [] ([],[]) emptyMemState. 
+   *)
+  Definition model_gen
+             (ret_typ : dtyp)
+             (entry : string)
+             (args : list uvalue)
+             (prog: list (toplevel_entity typ (block typ * list (block typ))))
+    : PropT L6 (MemState * (local_env * lstack * (global_env * uvalue))) :=
+    let t := denote_vellvm ret_typ entry args (convert_types (mcfg_of_tle prog)) in
+    ℑs eq t [] ([],[]) emptyMemState. 
 
-(**
+  (**
      Finally, the official model assumes no user-defined intrinsics.
- *)
-Definition model := model_gen (DTYPE_I 32%N) "main" main_args.
+   *)
+  Definition model := model_gen (DTYPE_I 32%N) "main" main_args.
+End Make.
