src/coq/Theory/InterpreterMCFG.v
@@ -11,184 +11,208 @@ From ITree Require Import
 From Vellvm Require Import
      Utilities
      Syntax
-     Semantics.
+     Semantics
+     Semantics.InterpretationStack.
 
 Import ITreeNotations.
-Import SemNotations.
-(* end hide *)
 
-(** * General facts on the MCFG-level interpretation
+Module MCFGTheory.
+  Declare Module TOP : LLVMTopLevel.
+
+  Export TOP.
+  Import SemNotations.
+  (* end hide *)
+
+  (** * General facts on the MCFG-level interpretation
   A collection of elementary facts about the interpretation when considering mcfgs
-*)
+   *)
 
-(* TO MOVE *)
-(* COMMON WITH CFG *)
-Arguments Intrinsics.F_trigger/.
-Arguments String.append : simpl never.
-Arguments allocate : simpl never.
-Arguments defs_assoc: simpl never.
+  (* TO MOVE *)
+  (* COMMON WITH CFG *)
+  Arguments Intrinsics.F_trigger/.
+  Arguments String.append : simpl never.
+  Arguments allocate : simpl never.
+  Arguments defs_assoc: simpl never.
 
-Module MCFGTactics.
-  (* Note: does not commute triggers for memory since those are more involved, we rely on specific lemmas *)
-  Ltac go :=
-    repeat match goal with
-           | |- context [interp_intrinsics (ITree.bind _ _)] => rewrite interp_intrinsics_bind
-           | |- context [interp_global (ITree.bind _ _)] => rewrite interp_global_bind
-           | |- context [interp_local_stack (ITree.bind _ _)] => rewrite interp_local_stack_bind
-           | |- context [interp_memory (ITree.bind _ _)] => rewrite interp_memory_bind
-           | |- context [interp_intrinsics (trigger _)] => rewrite interp_intrinsics_trigger; cbn; rewrite ?subevent_subevent
-           | |- context [interp_global (trigger _)] => rewrite interp_global_trigger; cbn; rewrite ?subevent_subevent
-           | |- context [interp_local_stack (trigger _)] => rewrite interp_local_stack_trigger; cbn; rewrite ?subevent_subevent
-           | |- context [ITree.bind (ITree.bind _ _) _] => rewrite bind_bind
-           | |- context [interp_intrinsics (Ret _)] => rewrite interp_intrinsics_ret
-           | |- context [interp_global (Ret _)] => rewrite interp_global_ret
-           | |- context [interp_local_stack (Ret _)] => rewrite interp_local_stack_ret
-           | |- context [interp_memory (Ret _)] => rewrite interp_memory_ret
-           | |- context [ITree.bind (Ret _) _] => rewrite bind_ret_l
-           end.
+  Module MCFGTactics.
+    (* Note: does not commute triggers for memory since those are more involved, we rely on specific lemmas *)
+    Ltac go :=
+      repeat match goal with
+             | |- context [interp_intrinsics (ITree.bind _ _)] => rewrite interp_intrinsics_bind
+             | |- context [interp_global (ITree.bind _ _)] => rewrite interp_global_bind
+             | |- context [interp_local_stack (ITree.bind _ _)] => rewrite interp_local_stack_bind
+             | |- context [interp_memory (ITree.bind _ _)] => rewrite interp_memory_bind
+             | |- context [interp_intrinsics (trigger _)] => rewrite interp_intrinsics_trigger; cbn; rewrite ?subevent_subevent
+             | |- context [interp_global (trigger _)] => rewrite interp_global_trigger; cbn; rewrite ?subevent_subevent
+             | |- context [interp_local_stack (trigger _)] => rewrite interp_local_stack_trigger; cbn; rewrite ?subevent_subevent
+             | |- context [ITree.bind (ITree.bind _ _) _] => rewrite bind_bind
+             | |- context [interp_intrinsics (Ret _)] => rewrite interp_intrinsics_ret
+             | |- context [interp_global (Ret _)] => rewrite interp_global_ret
+             | |- context [interp_local_stack (Ret _)] => rewrite interp_local_stack_ret
+             | |- context [interp_memory (Ret _)] => rewrite interp_memory_ret
+             | |- context [ITree.bind (Ret _) _] => rewrite bind_ret_l
+             end.
 
-End MCFGTactics.
+  End MCFGTactics.
 
-Import MCFGTactics.
+  Import MCFGTactics.
 
-Lemma interp1_bind :
-  forall {R S} (t: itree L0 R) (k: R -> itree L0 S) g, 
-    ℑs1 (t >>= k) g ≈ '(g',x) <- ℑs1 t g ;; ℑs1 (k x) g'.
-Proof.
-  intros; unfold ℑs1.
-  go.
-  apply eutt_eq_bind; intros (? & ?); reflexivity.
-Qed.
+  Lemma interp1_bind :
+    forall {R S} (t: itree L0 R) (k: R -> itree L0 S) g, 
+      ℑs1 (t >>= k) g ≈ '(g',x) <- ℑs1 t g ;; ℑs1 (k x) g'.
+  Proof.
+    intros; unfold ℑs1.
+    go.
+    apply eutt_eq_bind; intros (? & ?); reflexivity.
+  Qed.
 
-Lemma interp1_ret : forall (R : Type) g (x : R), ℑs1 (Ret x) g ≈ Ret1 g x.
-Proof.
-  intros; unfold ℑs1.
-  go; reflexivity.
-Qed.
+  Lemma interp1_ret : forall (R : Type) g (x : R), ℑs1 (Ret x) g ≈ Ret1 g x.
+  Proof.
+    intros; unfold ℑs1.
+    go; reflexivity.
+  Qed.
 
-Lemma interp2_bind :
-  forall {R S} (t: itree L0 R) (k: R -> itree L0 S) g l,
-    ℑs2 (t >>= k) g l ≈ '(g',(l',x)) <- ℑs2 t g l;; ℑs2 (k x) l' g'.
-Proof.
-  intros; unfold ℑs2.
-  go.
-  apply eutt_eq_bind; intros (? & ? & ?); reflexivity.
-Qed.
+  Lemma interp2_bind :
+    forall {R S} (t: itree L0 R) (k: R -> itree L0 S) g l,
+      ℑs2 (t >>= k) g l ≈ '(g',(l',x)) <- ℑs2 t g l;; ℑs2 (k x) l' g'.
+  Proof.
+    intros; unfold ℑs2.
+    go.
+    apply eutt_eq_bind; intros (? & ? & ?); reflexivity.
+  Qed.
 
-Lemma interp2_ret : forall (R : Type) g l (x : R), ℑs2 (Ret x) g l ≈ Ret2 g l x.
-Proof.
-  intros; unfold ℑs2.
-  go; reflexivity.
-Qed.
+  Lemma interp2_ret : forall (R : Type) g l (x : R), ℑs2 (Ret x) g l ≈ Ret2 g l x.
+  Proof.
+    intros; unfold ℑs2.
+    go; reflexivity.
+  Qed.
 
-Lemma interp3_bind :
-  forall {R S} (t: itree L0 R) (k: R -> itree L0 S) g l m,
-    ℑs3 (t >>= k) g l m ≈ '(m',(l',(g',x))) <- ℑs3 t g l m;; ℑs3 (k x) g' l' m'.
-Proof.
-  intros.
-  unfold ℑs3.
-  go.
-  apply eutt_eq_bind; intros (? & ? & ? & ?); reflexivity.
-Qed.
+  Lemma interp3_bind :
+    forall {R S} (t: itree L0 R) (k: R -> itree L0 S) g l m,
+      ℑs3 (t >>= k) g l m ≈ '(m',(l',(g',x))) <- ℑs3 t g l m;; ℑs3 (k x) g' l' m'.
+  Proof.
+    intros.
+    unfold ℑs3.
 
-Lemma interp3_ret : forall (R : Type) g l m (x : R), ℑs3 (Ret x) g l m ≈ Ret3 g l m x.
-Proof.
-  intros; unfold ℑs3.
-  go; reflexivity.
-Qed.
+    rewrite interp_intrinsics_bind.
+    rewrite interp_global_bind.
+    rewrite interp_local_stack_bind.
+    pose proof interp_memory_bind.
+    Import LLVM.MEMORY_THEORY.Mem.
+    cbn.
+    rewrite Vellvm.Theory.InterpreterMCFG.MCFGTheory.TOP.IS.LLVM.MEMORY_THEORY.interp_memory_bind.
+    go.
 
-#[global] Instance eutt_interp1 {T}:
-  Proper (eutt eq ==> eq ==> eutt eq) (@ℑs1 T).
-Proof.
-  repeat intro.
-  unfold ℑs1.
-  subst; rewrite H.
-  reflexivity.
-Qed.
 
-#[global] Instance eutt_interp2 {T}:
-  Proper (eutt eq ==> eq ==> eq ==> eutt eq) (@ℑs2 T).
-Proof.
-  repeat intro.
-  unfold ℑs2.
-  subst; rewrite H.
-  reflexivity.
-Qed.
+    pose proof Vellvm.Handlers.Handlers.MEMORY_THEORY.interp_memory_bind.
+    pose proof Vellvm.Theory.InterpreterMCFG.MCFGTheory.TOP.IS.LLVM.MEMORY_THEORY.interp_memory_bind.
+    pose proof Vellvm.Handlers.Handlers.MEMORY_THEORY64.interp_memory_bind.
 
-#[global] Instance eutt_interp3 {T}:
-  Proper (eutt eq ==> eq ==> eq ==> eq ==> eutt eq) (@ℑs3 T).
-Proof.
-  repeat intro.
-  unfold ℑs3.
-  subst; rewrite H.
-  reflexivity.
-Qed.
+    About Vellvm.Handlers.Handlers.MEMORY_THEORY.interp_memory_bind.
+    About Vellvm.Theory.InterpreterMCFG.MCFGTheory.TOP.IS.LLVM.MEMORY_THEORY.interp_memory_bind.
+    About Vellvm.Handlers.Handlers.MEMORY_THEORY64.interp_memory_bind.
 
-Lemma interp3_vis: 
-  forall T R (e : L0 T) (k : T -> itree L0 R) g l m,
-    ℑs3 (Vis e k) g l m ≈ 
-            '(m, (l, (g, x))) <- ℑs3 (trigger e) g l m;; ℑs3 (k x) g l m.
-Proof.
-  intros.
-  unfold ℑs3.
-  rewrite interp_intrinsics_vis.
-  go.
-  apply eutt_eq_bind.
-  intros (? & ? & ? & ?).
-  go.
-  reflexivity.
-Qed.
+    apply eutt_eq_bind; intros (? & ? & ? & ?); reflexivity.
+  Qed.
 
-Lemma interp3_bind_trigger :
-  forall T R (e : L0 T) (k : T -> itree L0 R) g l m,
-    ℑs3 (trigger e >>= k) g l m ≈ 
-            '(m, (l, (g, x))) <- ℑs3 (trigger e) g l m;; ℑs3 (k x) g l m.
-Proof.
-  intros.
-  rewrite bind_trigger.
-  rewrite interp3_vis at 1.
-  reflexivity.
-Qed.
+  Lemma interp3_ret : forall (R : Type) g l m (x : R), ℑs3 (Ret x) g l m ≈ Ret3 g l m x.
+  Proof.
+    intros; unfold ℑs3.
+    go; reflexivity.
+  Qed.
 
-Lemma interp3_GW : forall id g l m v,
-    ℑs3 (trigger (GlobalWrite id v)) g l m ≈ Ret3 (Maps.add id v g) l m tt.
-Proof.
-  intros.
-  unfold ℑs3.
-  go.
-  reflexivity.
-Qed.
+  #[global] Instance eutt_interp1 {T}:
+    Proper (eutt eq ==> eq ==> eutt eq) (@ℑs1 T).
+  Proof.
+    repeat intro.
+    unfold ℑs1.
+    subst; rewrite H.
+    reflexivity.
+  Qed.
 
-(* Lemma interp_cfg3_LM : forall t a prov g l (m : MemState) v, *)
-(*     deserialize_sbytes (lookup_all_index a (sizeof_dtyp t) bytes SUndef) t = v -> *)
-(*     ℑs3 (trigger (Load t (DVALUE_Addr (a, prov)))) g l m ≈ Ret3 g l m v. *)
-(* Proof. *)
-(*   intros * LUL EQ. *)
-(*   unfold ℑs3. *)
-(*   go. *)
-(*   rewrite interp_memory_load; cycle -1. *)
-(*   unfold read. *)
-(*   cbn in *; rewrite LUL; reflexivity. *)
-(*   go. *)
-(*   unfold read_in_mem_block; rewrite EQ. *)
-(*   reflexivity. *)
-(* Qed. *)
+  #[global] Instance eutt_interp2 {T}:
+    Proper (eutt eq ==> eq ==> eq ==> eutt eq) (@ℑs2 T).
+  Proof.
+    repeat intro.
+    unfold ℑs2.
+    subst; rewrite H.
+    reflexivity.
+  Qed.
 
-(* Lemma interp3_alloca : *)
-(*   forall (m : memory_stack) (t : dtyp) (g : global_env) l, *)
-(*     non_void t -> *)
-(*     exists m' a', *)
-(*       allocate m t = inr (m', a') /\ *)
-(*       ℑs3 (trigger (Alloca t)) g l m ≈ ret (m', (l, (g, DVALUE_Addr a'))). *)
-(* Proof. *)
-(*   intros * NV. *)
-(*   unfold ℑs3. *)
-(*   eapply interp_memory_alloca_exists in NV as [m' [a' [ALLOC INTERP]]]. *)
-(*   exists m', a'. *)
-(*   split; eauto. *)
-(*   go. *)
-(*   rewrite interp_memory_alloca; eauto. *)
-(*   go; reflexivity. *)
-(*   Unshelve. *)
-(*   auto. *)
-(* Qed. *)
+  #[global] Instance eutt_interp3 {T}:
+    Proper (eutt eq ==> eq ==> eq ==> eq ==> eutt eq) (@ℑs3 T).
+  Proof.
+    repeat intro.
+    unfold ℑs3.
+    subst; rewrite H.
+    reflexivity.
+  Qed.
+
+  Lemma interp3_vis: 
+    forall T R (e : L0 T) (k : T -> itree L0 R) g l m,
+      ℑs3 (Vis e k) g l m ≈ 
+          '(m, (l, (g, x))) <- ℑs3 (trigger e) g l m;; ℑs3 (k x) g l m.
+  Proof.
+    intros.
+    unfold ℑs3.
+    rewrite interp_intrinsics_vis.
+    go.
+    apply eutt_eq_bind.
+    intros (? & ? & ? & ?).
+    go.
+    reflexivity.
+  Qed.
+
+  Lemma interp3_bind_trigger :
+    forall T R (e : L0 T) (k : T -> itree L0 R) g l m,
+      ℑs3 (trigger e >>= k) g l m ≈ 
+          '(m, (l, (g, x))) <- ℑs3 (trigger e) g l m;; ℑs3 (k x) g l m.
+  Proof.
+    intros.
+    rewrite bind_trigger.
+    rewrite interp3_vis at 1.
+    reflexivity.
+  Qed.
+
+  Lemma interp3_GW : forall id g l m v,
+      ℑs3 (trigger (GlobalWrite id v)) g l m ≈ Ret3 (Maps.add id v g) l m tt.
+  Proof.
+    intros.
+    unfold ℑs3.
+    go.
+    reflexivity.
+  Qed.
+
+  (* Lemma interp_cfg3_LM : forall t a prov g l (m : MemState) v, *)
+  (*     deserialize_sbytes (lookup_all_index a (sizeof_dtyp t) bytes SUndef) t = v -> *)
+  (*     ℑs3 (trigger (Load t (DVALUE_Addr (a, prov)))) g l m ≈ Ret3 g l m v. *)
+  (* Proof. *)
+  (*   intros * LUL EQ. *)
+  (*   unfold ℑs3. *)
+  (*   go. *)
+  (*   rewrite interp_memory_load; cycle -1. *)
+  (*   unfold read. *)
+  (*   cbn in *; rewrite LUL; reflexivity. *)
+  (*   go. *)
+  (*   unfold read_in_mem_block; rewrite EQ. *)
+  (*   reflexivity. *)
+  (* Qed. *)
+
+  (* Lemma interp3_alloca : *)
+  (*   forall (m : memory_stack) (t : dtyp) (g : global_env) l, *)
+  (*     non_void t -> *)
+  (*     exists m' a', *)
+  (*       allocate m t = inr (m', a') /\ *)
+  (*       ℑs3 (trigger (Alloca t)) g l m ≈ ret (m', (l, (g, DVALUE_Addr a'))). *)
+  (* Proof. *)
+  (*   intros * NV. *)
+  (*   unfold ℑs3. *)
+  (*   eapply interp_memory_alloca_exists in NV as [m' [a' [ALLOC INTERP]]]. *)
+  (*   exists m', a'. *)
+  (*   split; eauto. *)
+  (*   go. *)
+  (*   rewrite interp_memory_alloca; eauto. *)
+  (*   go; reflexivity. *)
+  (*   Unshelve. *)
+  (*   auto. *)
+  (* Qed. *)
